ntt_base_case

crypto_examples/ntt.dfy
@@ -1,84 +1,257 @@
-include "../std_lib/src/NonlinearArithmetic/Power.dfy"
-include "../std_lib/src/NonlinearArithmetic/DivMod.dfy"
+include "pow2.dfy"
 
 module ntt {
     import opened Power
     import opened DivMod
+    import opened Mul
+    import opened pows_of_2
 
     const G: nat := 7 // 256-th root of unity
     const Q: nat := 12289
 
     type elem = i :nat | i < Q
 
-    // datatype elem = elem(n: nat, pow: nat)
-
-    function method modmul(a: elem, b: elem): elem
+    function method omega_n(n: pow2_t): elem
+        requires n.exp <= 8
     {
-        (a * b) % Q
+        Pow(G, Pow2(8 - n.exp)) % Q
     }
+
+    function method omega_nk(n: pow2_t, k: nat): elem
+        requires n.exp <= 8
+    {
+        Pow(omega_n(n), k) % Q
+    }
+
+    lemma mod_pow_cancel(b: nat, e: nat)
+        decreases e
+        ensures IsModEquivalent(Pow(b, e), Pow(b % Q, e), Q)
+    {
+        if e == 0 {
+            reveal Pow();
+            return;
+        }
+    
+        assert IsModEquivalent(Pow(b, e-1), Pow(b % Q, e-1), Q) by {
+            mod_pow_cancel(b, e-1);
+        }
+
+        assert IsModEquivalent(Pow(b, e-1) * b, Pow(b, e), Q) by {
+            reveal Pow();
+        }
+
+        assert IsModEquivalent(Pow(b % Q, e), Pow(b % Q, e-1) * (b % Q), Q) by {
+            reveal Pow();
+        }
+
+        assert IsModEquivalent(Pow(b, e-1) * b, Pow(b % Q, e-1) * b, Q) by {
+            LemmaModMulEquivalentAuto();
+        }
+
+        assert IsModEquivalent(Pow(b % Q, e-1) * b, Pow(b % Q, e-1) * (b % Q), Q) by {
+            assert IsModEquivalent(b, (b % Q), Q) by {
+                LemmaModBasicsAuto();
+            }
+            LemmaModMulEquivalent(b, (b % Q), Pow(b % Q, e-1), Q);
+        }
+    }
+
+    lemma omega_nk_canonical(n: pow2_t, k: nat)
+        requires n.exp <= 8
+        ensures Pow2(8 - n.exp) * k >= 0;   
+        ensures omega_nk(n, k) == Pow(G, Pow2(8 - n.exp) * k) % Q;
+    {
+        var om_nk := omega_nk(n, k);
+        var temp := Pow(G, Pow2(8 - n.exp));
+        LemmaPowPositiveAuto();
+
+        assert IsModEquivalent(Pow(temp, k), Pow(temp % Q, k), Q) by {
+            mod_pow_cancel(temp, k);
+        }
+
+        calc == {
+            om_nk;
+            Pow(omega_n(n), k) % Q;
+            Pow(temp % Q, k) % Q;
+            {
+                mod_pow_cancel(temp, k);
+            }
+            Pow(temp, k) % Q;
+            Pow(Pow(G, Pow2(8 - n.exp)), k) % Q;
+            {
+                LemmaPowMultiplies(G, Pow2(8 - n.exp), k);
+            }
+            Pow(G, Pow2(8 - n.exp) * k) % Q;
+        }
+
+        assert Pow2(8 - n.exp) * k >= 0 by {
+            LemmaMulStrictlyPositiveAuto();
+        }
+    }
+
+    lemma cancellation_lemma(n: pow2_t, k: nat)
+        requires n.exp != 0;
+        requires n.exp <= 8
+        ensures omega_nk(pow2_half(n), k) == omega_nk(n, 2 * k);
 
     function method modpow(a: elem, b: nat): elem
     {
         Pow(a, b) % Q
     }
 
-    function method Pow2(e: nat): nat
+    function method modmul(a: elem, b: elem): elem
     {
-        LemmaPowPositive(2, e);
-        Pow(2, e)
+        (a * b) % Q
     }
 
-    lemma Pow2Properties1(i: nat)
-        ensures i == 0 ==> Pow2(i) == 1;
-        ensures i == 1 ==> Pow2(i) == 2;
-        ensures i > 1 ==> Pow2(i) % 2 == 0;
-
-    lemma Pow2Properties2(i: nat, j: nat)
-        requires j <= i;
-        ensures 1 <= Pow(2, j);
-        ensures Pow(2, i) % Pow(2, j) == 0;
-
-    method fft(a: seq<elem>, logn: nat, omega: elem) returns (y: seq<elem>)
-        requires 1 <= |a| == Pow2(logn)
-        requires logn <= 8
-        requires |a| == 1 || |a| % 2 == 0
-        requires Pow2(8) % |a| == 0
-        requires omega == modpow(G, Pow2(8 - logn))
-        decreases logn
+    function method modadd(a: elem, b: elem): elem
     {
-        var len := |a|;
-        if |a| == 1 {
+        (a + b) % Q
+    }
+
+    function method modsub(a: elem, b: elem): elem
+    {
+        (a - b) % Q
+    }
+
+    function poly_eval(a: seq<elem>, x: elem): elem
+    // {
+    //     if |a| == 0
+    //         then 0
+    //     else
+    //         modadd(modpow(First(a), x), modmul(poly_eval(DropFirst(a), x), x))
+    // }
+
+    lemma poly_eval_split_lemma(a: seq<elem>, 
+        a_e: seq<elem>, a_o: seq<elem>, len': pow2_t, x: elem)
+        requires |a| == len'.full * 2;
+        requires a_e ==
+            seq(len'.full, n requires 0 <= n < len'.full => a[n * 2]);
+        requires a_o == 
+            seq(len'.full, n requires 0 <= n < len'.full => a[n * 2 + 1]);
+        ensures var sqr := modmul(x, x);
+            poly_eval(a, x)
+                == 
+            modadd(poly_eval(a_e, sqr), modmul(x, poly_eval(a_o, sqr)));
+
+    predicate poly_eval_all_points(a: seq<elem>, y: seq<elem>, len: pow2_t)
+        requires 0 <= len.exp <= 8
+    {
+        && |y| == |a| == len.full
+        && (forall i: nat :: i < len.full ==>
+            y[i] == poly_eval(a, omega_nk(len, i)))
+    }
+
+    // lemma y_k_correct(a: seq<elem>,
+    //     logn: nat,
+    //     a_e: seq<elem>, a_o: seq<elem>, len': nat,
+    //     omg_n: elem, omg_n': elem, k: nat,
+    //     y_e_k: elem, y_o_k: elem, y_k: elem)
+
+    //     requires |a| == len' * 2;
+    //     requires |a| == Pow2(logn);
+    //     requires k < len';
+    //     requires a_e == seq(len', n requires 0 <= n < len' => a[n * 2]);
+    //     requires a_o == seq(len', n requires 0 <= n < len' => a[n * 2 + 1]);
+    //     requires logn <= 8
+    //     requires omg_n == modpow(G, Pow2(8 - logn))
+    //     requires omg_n' == modpow(G, Pow2(8 - logn + 1))
+
+    //     requires y_e_k == poly_eval(a_e, modpow(omg_n', k));
+    //     requires y_o_k == poly_eval(a_o, modpow(omg_n', k));
+    //     requires y_k == modadd(y_e_k, modmul(modpow(omg_n, k), y_o_k));
+    // {
+    //     var sqr := modmul(modpow(omg_n, k), modpow(omg_n, k));
+        
+    //     calc == {
+    //         poly_eval(a, modpow(omg_n, k));
+    //         {
+    //             poly_eval_split_lemma(a, a_e, a_o, len', modpow(omg_n, k));
+    //         }
+    //         modadd(poly_eval(a_e, sqr), modmul(modpow(omg_n, k), poly_eval(a_o, sqr)));
+
+    //     }
+
+    //     // modadd(poly_eval(a_e, sqr), modmul(x, poly_eval(a_o, sqr)));
+    // }
+
+    lemma ntt_base_case(a: seq<elem>, len: pow2_t)
+        requires len.full == 1;
+        requires |a| == len.full;
+        ensures len.exp == 0;
+        ensures a[0] == poly_eval(a, omega_nk(len, 0));
+    {
+        pow2_basics(len);
+        assert len.exp == 0;
+
+        calc {
+            poly_eval(a, omega_nk(len, 0));
+            {
+                omega_nk_canonical(len, 0);
+                assert omega_nk(len, 0) == 
+                    Pow(G, Pow2(8 - len.exp) * 0) % Q;
+            }
+            poly_eval(a, Pow(G, Pow2(8 - len.exp) * 0) % Q);
+            poly_eval(a, Pow(G, 0) % Q);
+            {
+                LemmaPow0(G);
+            }
+            poly_eval(a, 1);
+            {
+                assume false; // TODO
+            }
+            a[0];
+        }
+
+    }
+
+    method ntt(a: seq<elem>, len: pow2_t) returns (y: seq<elem>)
+        requires 1 <= len.full;
+        requires len.exp <= 8;
+        requires |a| == len.full;
+        ensures poly_eval_all_points(a, y, len)
+        decreases len.full
+    {
+        if len.full == 1 {
+            ntt_base_case(a, len);
             return a;
         }
-        assert logn != 0 by {
-            LemmaPow0(2);
+
+        var len' := pow2_half(len);
+        var a_e := seq(len'.full, n requires 0 <= n < len'.full => a[n * 2]);
+        var a_o := seq(len'.full, n requires 0 <= n < len'.full => a[n * 2 + 1]);
+
+        var y_e := ntt(a_e, len');
+        // assert 
+        var y_o := ntt(a_o, len');
+
+        y := seq(len.full, n requires 0 <= n < len.full => 0);
+
+        var omgn := omega_n(len);
+        var omg := 1;
+        var k := 0;
+
+        while (k < len'.full)
+            invariant |y| == len.full;
+            // invariant 
+            decreases len'.full - k;
+        {
+            var y_e_k := y_e[k];
+            var y_o_k := y_o[k];
+
+            assert y_e_k == poly_eval(a_e, omega_nk(len', k));
+            assert y_o_k == poly_eval(a_o, omega_nk(len', k));
+
+            var y_k := modadd(y_e_k, modmul(omg, y_o_k));
+            y := y[k := y_k];
+
+            var y_k' := modsub(y_e_k, modmul(omg, y_o_k));
+            y := y[k + len'.full := y_k'];
+
+            omg := modmul(omg, omgn);
+            k := k + 1;
         }
-
-        assert Pow(2, logn-1) * 2 == Pow(2, logn) by {
-            reveal Pow();
-        }
-        var len' := len / 2;
-        var a_e := seq(len', n requires 0 <= n < len' => a[n * 2]);
-        var a_o := seq(len', n requires 0 <= n < len' => a[n * 2 + 1]);
-
-        var omega' := modmul(omega, omega);
-        assume omega' == modpow(G, Pow2(8 - logn + 1));
-
-        assert len' % 2 == 0 || len' == 1 by {
-            Pow2Properties1(logn - 1);
-        }
-
-        assert Pow2(8) % len' == 0 by {
-            Pow2Properties2(8, logn - 1);
-        }
-
-
-        var y_e := fft(a_e, logn-1, omega');
-        var y_o := fft(a_o, logn-1, omega');
-        
-        // var omega := 
+        assume false;
     }
-
-
 }
 
