crypto_examples/pow2.dfy
@@ -1,0 +1,109 @@
+include "../std_lib/src/NonlinearArithmetic/Power.dfy"
+include "../std_lib/src/NonlinearArithmetic/DivMod.dfy"
+include "../std_lib/src/Collections/Sequences/Seq.dfy"
+
+module pows_of_2 {
+    import opened Power
+    import opened DivMod
+    import opened Mul
+
+    function method Pow2(e: nat): nat
+    {
+        LemmaPowPositive(2, e);
+        Pow(2, e)
+    }
+
+    datatype pow2_t_raw = pow2_t_cons(full: nat, exp: nat)
+
+    type pow2_t = n: pow2_t_raw | n.full == Pow2(n.exp) witness *
+
+    function pow2(exp: nat): pow2_t
+    {
+        LemmaPowPositiveAuto();
+        pow2_t_cons(Pow(2, exp), exp)
+    }
+
+    lemma pow2_basics(n: pow2_t)
+        ensures n.exp == 0 ==> n.full == 1
+        ensures n.exp != 0 ==> n.full % 2 == 0
+    {
+        reveal Pow();
+    }
+
+    // lemma pow2_double(n: pow2_t) returns (n': pow2_t)
+    //     ensures n'.exp == n.exp + 1
+    //     ensures n'.full == 2 * n.full
+    // {
+    //     var m := pow2_t_cons(2 * n.full, n.exp + 1);
+
+    //     calc == {
+    //         m.full;
+    //         2 * n.full;
+    //         2 * Pow2(n.exp);
+    //         {
+    //             reveal Pow();
+    //         }
+    //         Pow2(n.exp + 1);
+    //         Pow2(m.exp);
+    //     }
+
+    //     n' := m;
+    // }
+
+    function method pow2_half(n: pow2_t) : (n': pow2_t)
+        requires n.exp != 0 || n.full != 1;
+        ensures n'.exp == n.exp - 1;
+        ensures n'.full * 2 == n.full;
+        ensures n.full % 2 == 0;
+        ensures n'.full == n.full / 2;
+    {
+        pow2_basics(n);
+        assert n.exp - 1 >= 0;
+        var m := pow2_t_cons(n.full / 2, n.exp - 1);
+        pow2_half_value_lemma(n, m);
+        m
+    }
+
+    lemma pow2_half_value_lemma(n: pow2_t, n': pow2_t_raw)
+        requires n.exp != 0;
+        requires n' == pow2_t_cons(n.full / 2, n.exp - 1);
+        ensures n'.exp == n.exp - 1;
+        ensures n'.full * 2 == n.full
+        ensures n'.full == Pow2(n'.exp);
+    {
+        pow2_basics(n);
+        // var m := pow2_t_cons(n.full / 2, n.exp - 1);
+
+        calc == {
+            n'.full;
+            n.full / 2;
+            Pow2(n.exp) / 2;
+            {
+                reveal Pow();
+            }
+            Pow2(n.exp - 1);
+            Pow2(n'.exp);
+        }
+    }
+
+    // lemma pow2_square(n: pow2_t) returns (n': pow2_t)
+    //     ensures n'.exp == 2 * n.exp 
+    //     ensures n'.full == n.full * n.full
+    // {
+    //     LemmaMulStrictlyPositiveAuto();
+    //     var m := pow2_t_cons(n.full * n.full, 2 * n.exp);
+
+    //     calc == {
+    //         m.full;
+    //         n.full * n.full;
+    //         Pow2(n.exp) * Pow2(n.exp);
+    //         {
+    //             LemmaPowAdds(2, n.exp, n.exp);
+    //         }
+    //         Pow2(n.exp + n.exp);
+    //         Pow2(m.exp);
+    //     }
+
+    //     n' := m;
+    // }
+}
